src/voteprivacy/applyDestrEnc.v
@@ -1,0 +1,90 @@
+(************************************************************************) 
+(* Copyright (c) 2017-2018, Ajay Kumar Eeralla <ae266@mail.missouri.edu>*)
+(************************************************************************)
+        
+Require Export auxDefs.
+   
+Proposition destrEnc:
+      let v0 := V0 (f (toListm phi0)) in
+      let v1 := V1 (f (toListm phi0)) in
+      (vcheck v0) & (vcheck v1) ## TRue ->
+      (* Bothsides *)
+      let r0 := (r 1) in
+      let r1 := (r 2) in
+      let k0 := (kc (nonce 3)) in
+      let k1 := (kc (nonce 4)) in
+      (* Left-side *)
+      let c00 := (comm v0 k0) in
+      let c11 := (comm v1 k1) in
+      let t := pubkey (f (toListm phi0)) in
+      let b00 := (bl c00 t r0) in
+      let b11 := (bl c11 t r1) in
+      let t0 := (((vk 0), (Mvar 5), sign (Mvar 5) (ssk 0) (sr 14)), ((vk 1), (Mvar 6), sign (Mvar 6) (ssk 1) (sr 15))) in
+      let t1 := (t0, f (cons t0 nil)) in
+      let t2 := ({{ 5 := (bl c00 t r0) }} ({{ 6:=(bl c11 t r1) }} t0)) in
+      let t3 := ({{ 5 := (bl c00 t r0) }} ({{ 6:=(bl c11 t r1) }} t1)) in
+      let acc00 := (acc c00 t r0 t2) in
+      let acc11 := (acc c11 t r1 t3) in
+      let e00 := (enc ((c00, ((ub c00 t r0 t2), (nonce 20))), TWO) (pke 11) (er 7)) in
+      let e11 := (enc ((c11, ((ub c11 t r1 t3), (nonce 21))), TWO) (pke 11) (er 8)) in
+      let phi02:= [msg b00, msg b11, msg e00, msg e11] in
+      let fphi02:= f (toListm phi02) in
+      let pv00 := (c00, ((ub c00 t r0 t2), (nonce 20))) in
+      let pv11 := (c11, ((ub c11 t r1 t3), (nonce 21))) in
+      let s0 := (If (! (isin pv00 ((pi1 (d 1 fphi02)), ((pi1 (d 2 fphi02)), (pi1 (d 3 fphi02)))))) then (shufl (pi1 (d 1 fphi02)) (pi1 (d 2 fphi02)) (pi1 (d 3 fphi02))) else O)in
+      let dv0 := (If (dist fphi02) & (pvchecks fphi02) then s0 else |_) in
+      let t0s0 := (If acc00 & acc11 then (e00, (e11, dv0)) else |_) in
+
+      (* Right-side *)
+      let c10 := (comm v1 k0) in
+      let c01 := (comm v0 k1) in 
+      let b10 := (bl c10 t r0) in
+      let b01 := (bl c01 t r1) in
+      let t4 := ({{ 5 := (bl c10 t r0) }} ({{ 6:=(bl c01 t r1) }} t0)) in
+      let t5 := ({{ 5 := (bl c10 t r0) }} ({{ 6:=(bl c01 t r1) }} t1)) in
+      let acc10 := (acc c10 t r0 t4) in
+      let acc01 := (acc c01 t r1 t5) in
+      let e10 := (enc ((c10, ((ub c10 t r0 t4), (nonce 20))), TWO) (pke 11) (er 7)) in
+      let e01 := (enc ((c01, ((ub c01 t r1 t5), (nonce 21))), TWO) (pke 11) (er 8)) in
+      let pv10 := (c10, ((ub c10 t r0 t4), (nonce 20))) in
+      let pv01 := (c01, ((ub c01 t r1 t5), (nonce 21))) in
+      let phi12:= [msg b10, msg b01, msg e10, msg e01] in
+      let fphi12:= f (toListm phi12) in
+      let s1 := (If (! (isin pv10 ((pi1 (d 1 fphi12)), ((pi1 (d 2 fphi12)), (pi1 (d 3 fphi12)))))) then (shufl (pi1 (d 1 fphi12)) (pi1 (d 2 fphi12)) (pi1 (d 3 fphi12))) else O)in
+      let dv1 := (If (dist fphi12) & (pvchecks fphi12) then s1 else |_) in
+      let t1s1 := (If acc10 & acc01 then (e10, (e01, dv1)) else |_) in 
+ 
+      [msg b00, msg b11, msg t0s0] ~ [msg b10, msg b01, msg t1s1].
+Proof. intros.
+       aply_cca2Trans (let e00' := (enc ((c00, ((ub c00 t r0 t2), (nonce 100))), TWO) (pke 11) (er 7)) in
+               let phi02':= [msg b00, msg b11, msg e00', msg e11] in
+               let fphi02':= f (toListm phi02') in
+               let s0' := (If (! (isin pv00 ((pi1 (d 1 fphi02')), ((pi1 (d 2 fphi02')), (pi1 (d 3 fphi02')))))) then (shufl (pi1 (d 1 fphi02')) (pi1 (d 2 fphi02')) (pi1 (d 3 fphi02'))) else O)in
+                                              let dv0' := (If (dist fphi02') & (pvchecks fphi02') then s0' else |_) in
+                                              let t0s0' := (If acc00 & acc11 then (e00', (e11, dv0')) else |_) in
+                                              [msg b00, msg b11, msg t0s0'])
+
+                ( let e10' := (enc ((c10, ((ub c10 t r0 t4), (nonce 100))), TWO) (pke 11) (er 7)) in
+                  let phi12':= [msg b10, msg b01, msg e10', msg e01] in
+      let fphi12':= f (toListm phi12') in
+      let s1' := (If (! (isin pv10 ((pi1 (d 1 fphi12')), ((pi1 (d 2 fphi12')), (pi1 (d 3 fphi12')))))) then (shufl (pi1 (d 1 fphi12')) (pi1 (d 2 fphi12')) (pi1 (d 3 fphi12'))) else O)in
+      let dv1' := (If (dist fphi12') & (pvchecks fphi12') then s1' else |_) in
+      let t1s1' := (If acc10 & acc01 then (e10', (e01, dv1')) else |_) in
+      [msg b10, msg b01, msg t1s1']).
+                      simpl.
+                      apply aplyCCA with (a:= 11) (r:= 7).
+                      simpl. reflexivity.
+                      simpl.
+apply nodup. simpl.
+                      aplyDestrEnc 11 7.
+      apply nodup.
+       simpl. simpl. unfold d. Compute destrEncMsg 11 (pi2 (dec (tau 3 fphi02) (ske 11))) (pi2 (dec (tau 3 O) (ske 11))).
+       (dec
+          (tau 3
+             (f
+                (b00
+                 :: b11
+                    :: {(c00, (ub c00 t r0 t2, nonce 100), TWO) }_ 11 ^^ 7
+                       :: e11 :: nil))) (ske 11))).
+Qed.
+       
